\documentclass{article}
\usepackage{amssymb}
\usepackage{url}
\usepackage{hyperref}

\def\Z\{mathbb{Z}

\newtheorem{theorem}{Theorem}
\newtheorem{proof}{Proof}

\begin{document}

\begin{center}
More Math in \LaTeX{} \\
Monday, January 27, 2014
\end{center}

\begin{theorem}
Let G be an abelian group and let $$c^n = c*c*c*...*c \mbox{ for $n$ factors $c$} $$, 
where $c \in G$ and $n \in Z^+$ (positive integers). Give a mathematical 
induction proof that 
\begin{eqnarray}
(a*b)^n = (a^n)*(b^n) \forall a,b \in G
\end{eqnarray}
\end{theorem}

New example from the Practice.pdf on BlackBoard
% * on eqnarray gives no numbers
\begin{eqnarray*}
\frac{dx_1}{dt} & = & x_1 - 2x_2 \\
\frac{dx_1}{dt} & = & 5x_1 - x_2
\end{eqnarray*}
More words here
%\begin{eqnarray*}
%    \det(A - \lambda I) & = & 
%    \det 
%    \left( \left[ 
%    \begin{array}{cc}
%    (1 - \lambda I) & -2 \\
%    5 & (-1 - \lambda)
%    \end{array}
%    \right] \right) \\
%    & = & (1 - \lambda) (-1 - \lambda) + 10 \\
%    & = & \lambda^2 + 9 \\
%    \mbox{ so, } \lambda $ = $ \pm 3 i
%\end{eqnarray}

\end{document}
